added a generic big-step semantics   (opsem.Opsem.bInsn, from ssa_dyanmic.LLVMopsem.dInsn), proved it simulates the small-step (opsem_props.OpsemConv, from opsem_conv.v), and it preserves uniqueness and inclusion (opsem_props.OpsemProps, from opsem_pp.v).
git-svn-id: https://webdav.seas.upenn.edu/svn/sol/vol@3206 eef5ea85-cc2e-0410-bd84-0fae1f012da8

src/ssa/opsem_props.v
@@ -25,6 +25,519 @@ Require Import AST.
 Require Import Maps.
 Require Import opsem.
 
+Module OpsemConv (GVsSig : GenericValuesSig).
+
+Module OPSEM := Opsem GVsSig.
+Export OPSEM.
+
+Lemma func_callUpdateLocals_is_returnUpdateLocals : 
+  forall TD rid noret0 tailc0 ft fid lp Result lc lc' gl,
+  returnUpdateLocals TD (insn_call rid noret0 tailc0 ft fid lp) Result 
+    lc lc' gl =
+  callUpdateLocals TD ft noret0 rid (Some Result) lc' lc gl.
+Proof.
+  intros.
+  unfold returnUpdateLocals. 
+  unfold callUpdateLocals.
+  destruct noret0; auto.
+Qed.
+
+Lemma proc_callUpdateLocals_is_id : forall TD ft rid noret0 lc lc' gl lc'',
+  callUpdateLocals TD ft noret0 rid None lc' lc gl = Some lc'' -> 
+  lc' = lc'' /\ noret0 = true.
+Proof.
+  intros.
+  unfold callUpdateLocals in H. 
+  destruct noret0; inversion H; auto.
+Qed.
+
+Lemma sInsn__implies__sop_star : forall state state' tr,
+  sInsn state state' tr ->
+  sop_star state state' tr.
+Proof.
+  intros state state' tr HdsInsn.
+  rewrite <- trace_app_nil__eq__trace.
+  eauto.
+Qed.
+
+Lemma sInsn__implies__sop_plus : forall state state' tr,
+  sInsn state state' tr ->
+  sop_plus state state' tr.
+Proof.
+  intros state state' tr HdsInsn.
+  rewrite <- trace_app_nil__eq__trace.
+  eauto.
+Qed.
+
+Lemma sop_plus__implies__sop_star : forall state state' tr,
+  sop_plus state state' tr ->
+  sop_star state state' tr.
+Proof.
+  intros state state' tr Hdsop_plus.
+  inversion Hdsop_plus; subst; eauto.
+Qed.
+
+Hint Resolve sInsn__implies__sop_star sInsn__implies__sop_plus 
+  sop_plus__implies__sop_star. 
+
+Lemma sop_star_trans : forall state1 state2 state3 tr12 tr23,
+  sop_star state1 state2 tr12 ->
+  sop_star state2 state3 tr23 ->
+  sop_star state1 state3 (trace_app tr12 tr23).
+Proof.
+  intros state1 state2 state3 tr12 tr23 Hdsop12 Hdsop23.
+  generalize dependent state3.
+  generalize dependent tr23.
+  induction Hdsop12; intros; auto.
+    rewrite <- trace_app_commute. eauto.
+Qed.
+
+Lemma sop_diverging_trans : forall state tr1 state' tr2,
+  sop_star state state' tr1 ->
+  sop_diverges state' tr2 ->
+  sop_diverges state (Trace_app tr1 tr2).
+Proof. 
+  intros state tr1 state' tr2 state_dsop_state' state'_dsop_diverges.
+  generalize dependent tr2.
+  (sop_star_cases (induction state_dsop_state') Case); intros; auto.
+  Case "sop_star_cons".
+    rewrite <- Trace_app_commute. eauto.
+Qed.
+
+(***********************************************************)
+(** big-step convergence -> small-step convergence *)
+
+(** First, by mutual induction, we prove that bInsn, bop and  
+    bFdef imply small-step semantics. *)
+
+Definition bInsn__implies__sop_plus_prop state state' tr 
+  (db:bInsn state state' tr) := sop_plus state state' tr.
+Definition bop__implies__sop_star_prop state state' tr (db:bop state state' tr) 
+  := sop_star state state' tr.
+Definition bFdef__implies__sop_star_prop fv rt lp S TD Ps ECs lc gl fs Mem lc'
+als' Mem' B'' rid oResult tr 
+(db:bFdef fv rt lp S TD Ps ECs lc gl fs Mem lc' als' Mem' B'' rid oResult tr) 
+  := 
+  match oResult with
+  | Some Result => forall fptrs,
+    getOperandValue TD fv lc gl = Some fptrs -> 
+    exists fptr, exists fa, exists fid, exists la, exists va, exists lb, 
+    exists l', exists ps', exists cs', exists tmn', exists gvs, exists lc0, 
+    fptr @ fptrs /\
+    lookupFdefViaPtr Ps fs fptr = 
+      Some (fdef_intro (fheader_intro fa rt fid la va) lb) /\
+    getEntryBlock (fdef_intro (fheader_intro fa rt fid la va) lb) = 
+      Some (block_intro l' ps' cs' tmn') /\
+    params2GVs TD lp lc gl = Some gvs /\
+    initLocals TD la gvs = Some lc0 /\
+    sop_star
+      (mkState S TD Ps ((mkEC (fdef_intro (fheader_intro fa rt fid la va) lb) 
+                              (block_intro l' ps' cs' tmn') cs' tmn' 
+                              lc0
+                               nil)::ECs) gl fs Mem)
+      (mkState S TD Ps ((mkEC (fdef_intro (fheader_intro fa rt fid la va) lb) 
+                               B'' nil (insn_return rid rt Result) lc'
+                               als')::ECs) gl fs 
+                               Mem')
+      tr
+  | None => forall fptrs,
+    getOperandValue TD fv lc gl = Some fptrs -> 
+    exists fptr, exists fa, exists fid, exists la, exists va, exists lb, 
+    exists l', exists ps', exists cs', exists tmn', exists gvs, exists lc0, 
+    fptr @ fptrs /\
+    lookupFdefViaPtr Ps fs fptr = 
+      Some (fdef_intro (fheader_intro fa rt fid la va) lb) /\
+    getEntryBlock (fdef_intro (fheader_intro fa rt fid la va) lb) = 
+      Some (block_intro l' ps' cs' tmn') /\
+    params2GVs TD lp lc gl = Some gvs /\
+    initLocals TD la gvs = Some lc0 /\
+    sop_star
+      (mkState S TD Ps ((mkEC (fdef_intro (fheader_intro fa rt fid la va) lb) 
+                              (block_intro l' ps' cs' tmn') cs' tmn' 
+                              lc0
+                              nil)::ECs) gl fs Mem)
+      (mkState S TD Ps ((mkEC (fdef_intro (fheader_intro fa rt fid la va) lb) 
+                               B'' nil (insn_return_void rid) lc'
+                               als')::ECs) gl fs 
+                               Mem')
+      tr
+  end
+  .
+
+Lemma b__implies__s:
+  (forall state state' t  db, @bInsn__implies__sop_plus_prop state state' t db)
+    /\
+  (forall state state' t  db, @bop__implies__sop_star_prop state state' t db) 
+    /\
+  (forall fv rt lp S TD Ps ECs lc gl fs Mem lc' als' Mem' B'' rid oret tr db, 
+     @bFdef__implies__sop_star_prop fv rt lp S TD Ps ECs lc gl fs Mem lc' als' 
+       Mem' B'' rid oret tr db).
+Proof.
+(b_mutind_cases
+  apply b_mutind with
+    (P  := bInsn__implies__sop_plus_prop)
+    (P0 := bop__implies__sop_star_prop)
+    (P1 := bFdef__implies__sop_star_prop)
+    Case);
+  unfold bInsn__implies__sop_plus_prop, 
+         bop__implies__sop_star_prop, 
+         bFdef__implies__sop_star_prop; 
+  intros; subst; simpl; intuition; eauto.
+  Case "bCall".
+    inversion b; subst.
+    SCase "bFdef_func".
+    assert (Hlookup:=H0).
+    apply H in H0; auto. clear H.
+    destruct H0 as [fptr' [fa0 [fid0 [la0 [va0 [lb0 [l0 [ps0 [cs0 [tmn0 [gvs0 
+      [lc0 [J1 [J2 [J3 [J4 [J5 J6]]]]]]]]]]]]]]]]].
+    rewrite <- nil_app_trace__eq__trace.
+    apply sop_plus_cons with 
+      (state2:=mkState S TD Ps 
+                      ((mkEC (fdef_intro (fheader_intro fa0 rt fid0 la0 va0) lb0)
+                               (block_intro l0 ps0 cs0 tmn0) cs0 tmn0 lc0
+                               nil)::
+                        (mkEC F B ((insn_call rid noret0 ca ft fv lp)::cs) 
+                         tmn lc als)::EC) 
+                        gl fs Mem0); eauto.
+    rewrite <- trace_app_nil__eq__trace.
+    apply sop_star_trans with 
+      (state2:=mkState S TD Ps 
+                     ((mkEC (fdef_intro (fheader_intro fa0 rt fid0 la0 va0) lb0)
+                               (block_intro l'' ps'' cs'' 
+                                (insn_return Rid rt Result)) nil 
+                                (insn_return Rid rt Result) lc'
+                                als')::
+                        (mkEC F B ((insn_call rid noret0 ca ft fv lp)::cs) 
+                         tmn lc als)::EC) 
+                         gl fs Mem'); auto.
+      apply sInsn__implies__sop_star.
+        apply sReturn; auto.
+          erewrite func_callUpdateLocals_is_returnUpdateLocals; eauto.
+
+    SCase "bFdef_proc".
+    assert (Hlookup:=H0).
+    apply H in H0; auto. clear H.
+    destruct H0 as [fptr' [fa0 [fid0 [la0 [va0 [lb0 [l0 [ps0 [cs0 [tmn0 [gvs0 
+      [lc0 [J1 [J2 [J3 [J4 [J5 J6]]]]]]]]]]]]]]]]].
+    rewrite <- nil_app_trace__eq__trace.
+    apply sop_plus_cons with 
+      (state2:=mkState S TD Ps 
+                      ((mkEC (fdef_intro (fheader_intro fa0 rt fid0 la0 va0) lb0)
+                               (block_intro l0 ps0 cs0 tmn0) cs0 tmn0 lc0
+                               nil)::
+                        (mkEC F B ((insn_call rid noret0 ca ft fv lp)::cs) 
+                         tmn lc als)::EC) 
+                        gl fs Mem0); eauto.
+    rewrite <- trace_app_nil__eq__trace.
+    apply proc_callUpdateLocals_is_id in e0.
+    destruct e0; subst.
+    apply sop_star_trans with 
+      (state2:=mkState S TD Ps 
+                      ((mkEC (fdef_intro (fheader_intro fa0 rt fid0 la0 va0) lb0)
+                               (block_intro l'' ps'' cs'' (insn_return_void Rid))
+                                nil (insn_return_void Rid) lc'
+                                als')::
+                        (mkEC F B ((insn_call rid true ca ft fv lp)::cs) 
+                         tmn lc'' als)::EC) 
+                        gl fs Mem'); auto.
+
+  Case "bop_cons".
+    apply sop_star_trans with (state2:=S2); auto.
+        
+  Case "bFdef_func".
+    rewrite H0 in e. inv e. exists fptr. exists fa. exists fid. exists la.
+    exists va. exists lb. exists l'. exists ps'. exists cs'. exists tmn'. 
+    exists gvs. exists lc0. repeat (split; auto).
+
+  Case "bFdef_proc".
+   rewrite H0 in e. inv e. exists fptr. exists fa. exists fid. exists la.
+    exists va. exists lb. exists l'. exists ps'. exists cs'. exists tmn'. 
+    exists gvs. exists lc0. repeat (split; auto).
+Qed.  
+    
+Lemma bInsn__implies__sop_plus : forall state state' tr,
+  bInsn state state' tr ->
+  sop_plus state state' tr.
+Proof.
+  destruct b__implies__s as [J _]. eauto.
+Qed.
+
+Lemma bInsn__implies__sop_star : forall state state' tr,
+  bInsn state state' tr ->
+  sop_star state state' tr.
+Proof. 
+  intros state state' tr state_dbInsn_state'.
+  apply bInsn__implies__sop_plus in state_dbInsn_state'; auto.
+Qed.
+
+Lemma bop__implies__sop_star : forall state state' tr,
+  bop state state' tr ->
+  sop_star state state' tr.
+Proof.
+  destruct b__implies__s as [_ [J _]]. eauto.
+Qed.
+
+Lemma bFdef_func__implies__sop_star : forall fv rt lp S TD Ps ECs lc gl fs
+    Mem lc' als' Mem' B'' rid Result tr fptrs, 
+  bFdef fv rt lp S TD Ps ECs lc gl fs Mem lc' als' Mem' B'' rid (Some Result) 
+    tr ->
+  getOperandValue TD fv lc gl = Some fptrs -> 
+  exists fptr, exists fa, exists fid, exists la, exists va, exists lb, 
+  exists l', exists ps', exists cs', exists tmn', exists gvs, exists lc0, 
+  fptr @ fptrs /\
+  lookupFdefViaPtr Ps fs fptr = 
+    Some (fdef_intro (fheader_intro fa rt fid la va) lb) /\
+  getEntryBlock (fdef_intro (fheader_intro fa rt fid la va) lb) = 
+    Some (block_intro l' ps' cs' tmn') /\
+  params2GVs TD lp lc gl = Some gvs /\
+  initLocals TD la gvs = Some lc0 /\
+  sop_star 
+    (mkState S TD Ps ((mkEC (fdef_intro (fheader_intro fa rt fid la va) lb) 
+                             (block_intro l' ps' cs' tmn') cs' tmn' lc0
+                             nil)::ECs) gl fs Mem)
+    (mkState S TD Ps ((mkEC (fdef_intro (fheader_intro fa rt fid la va) lb) 
+                             B'' nil (insn_return rid rt Result) lc'
+                             als')::ECs) gl fs Mem')
+    tr.
+Proof.
+  intros fv rt lp S TD Ps EC lc gl fs Mem0 lc' als' Mem' B'' rid Result tr 
+    fptrs H H1.
+  destruct b__implies__s as [_ [_ J]]. 
+  assert (K:=@J fv rt lp S TD Ps EC lc gl fs Mem0 lc' als' Mem' B'' rid 
+    (Some Result) tr H fptrs H1); auto.
+Qed.
+
+Lemma bFdef_proc__implies__sop_star : forall fv rt lp S TD Ps ECs lc gl fs
+    Mem lc' als' Mem' B'' rid tr fptrs,
+  bFdef fv rt lp S TD Ps ECs lc gl fs  Mem lc' als' Mem' B'' rid None tr ->
+  getOperandValue TD fv lc gl = Some fptrs -> 
+  exists fptr, exists fa, exists fid, exists la, exists va, exists lb, 
+  exists l', exists ps', exists cs', exists tmn', exists gvs, exists lc0, 
+  fptr @ fptrs /\
+  lookupFdefViaPtr Ps fs fptr = 
+    Some (fdef_intro (fheader_intro fa rt fid la va) lb) /\
+  getEntryBlock (fdef_intro (fheader_intro fa rt fid la va) lb) = 
+    Some (block_intro l' ps' cs' tmn') /\
+  params2GVs TD lp lc gl = Some gvs /\
+  initLocals TD la gvs = Some lc0 /\
+  sop_star 
+    (mkState S TD Ps ((mkEC (fdef_intro (fheader_intro fa rt fid la va) lb) 
+                            (block_intro l' ps' cs' tmn') cs' tmn' lc0
+                            nil)::ECs) gl fs Mem)
+    (mkState S TD Ps ((mkEC (fdef_intro (fheader_intro fa rt fid la va) lb) 
+                             B'' nil (insn_return_void rid) lc'
+                             als')::ECs) gl fs Mem')
+    tr.
+Proof.
+  intros fv rt lp S TD Ps EC lc gl fs Mem0 lc' als' Mem' B'' rid tr fptrs H H1.
+  destruct b__implies__s as [_ [_ J]]. 
+  assert (K:=@J fv rt lp S TD Ps EC lc gl fs Mem0 lc' als' Mem' B'' rid None tr 
+    H fptrs H1); auto.
+Qed.
+
+(** Then we prove that the whole program holds the same property. *)
+
+Lemma b_converges__implies__s_converges : forall sys main VarArgs FS,
+  b_converges sys main VarArgs FS ->
+  s_converges sys main VarArgs FS.
+Proof.
+  intros sys main VarArgs FS Hdb_converges.
+  inversion Hdb_converges; subst.
+  apply s_converges_intro with (IS:=IS)(tr:=tr); auto.
+  apply bop__implies__sop_star; auto.
+Qed.
+
+Lemma b_goeswrong__implies__s_goeswrong : forall sys main VarArgs FS,
+  b_goeswrong sys main VarArgs FS ->
+  s_goeswrong sys main VarArgs FS.
+Proof.
+  intros sys main VarArgs FS Hdb_goeswrong.
+  inversion Hdb_goeswrong; subst.
+  apply s_goeswrong_intro with (IS:=IS)(tr:=tr); auto.
+  apply bop__implies__sop_star; auto.
+Qed.
+
+(***********************************************************)
+(** big-step divergence -> small-step divergence *)
+
+(** First,we prove that bInsn, bop and bFdef imply small-step semantics,
+    by nested coinduction. *)
+
+Lemma bFdefInf_bopInf__implies__sop_diverges : 
+   forall (fv : value) (rt : typ) (lp : params) (S : system)
+     (TD : TargetData) (Ps : products) (ECs : list ExecutionContext)
+     (lc : GVsMap) (gl fs : GVMap) (Mem0 : mem) (tr : Trace) 
+     (fid : id) (fa : fnattrs) (lc1 : GVsMap) (l' : l) 
+     (ps' : phinodes) (cs' : cmds) (tmn' : terminator) 
+     (la : args) (va : varg) (lb : blocks) (gvs : list GVs) 
+     (fptrs0 : GVs) (fptr : GenericValue),
+   fptr @ fptrs0 ->
+   lookupFdefViaPtr Ps fs fptr =
+   ret fdef_intro (fheader_intro fa rt fid la va) lb ->
+   getEntryBlock (fdef_intro (fheader_intro fa rt fid la va) lb) =
+   ret block_intro l' ps' cs' tmn' ->
+   params2GVs TD lp lc gl = ret gvs ->
+   initLocals TD la gvs = ret lc1 ->
+   bopInf
+     {|
+     CurSystem := S;
+     CurTargetData := TD;
+     CurProducts := Ps;
+     ECS := {|
+            CurFunction := fdef_intro (fheader_intro fa rt fid la va) lb;
+            CurBB := block_intro l' ps' cs' tmn';
+            CurCmds := cs';
+            Terminator := tmn';
+            Locals := lc1;
+            Allocas := nil |} :: ECs;
+     Globals := gl;
+     FunTable := fs;
+     Mem := Mem0 |} tr ->
+   getOperandValue TD fv lc gl = ret fptrs0 ->
+   sop_diverges
+     {|
+     CurSystem := S;
+     CurTargetData := TD;
+     CurProducts := Ps;
+     ECS := {|
+            CurFunction := fdef_intro (fheader_intro fa rt fid la va) lb;
+            CurBB := block_intro l' ps' cs' tmn';
+            CurCmds := cs';
+            Terminator := tmn';
+            Locals := lc1;
+            Allocas := nil |} :: ECs;
+     Globals := gl;
+     FunTable := fs;
+     Mem := Mem0 |} tr.
+Proof.
+  cofix CIH_bFdefInf.
+
+  assert (forall state tr, 
+          bInsnInf state tr -> 
+          sop_diverges state tr) as bInsnInf__implies__sop_diverges.
+    cofix CIH_bInsnInf.
+    intros state tr HbInsnInf.
+    
+    inversion HbInsnInf; subst.
+    rewrite <- nil_app_Trace__eq__Trace.
+    assert (HbFdefInf:=H).
+    inversion H; subst.
+    apply sop_diverges_intro with 
+      (state2:=mkState S TD Ps 
+                       ((mkEC (fdef_intro (fheader_intro fa rt fid la va)lb)
+                               (block_intro l' ps' cs' tmn') cs' tmn' lc1
+                               nil)::
+                        (mkEC F B ((insn_call rid noret0 ca ft fv lp)::cs) 
+                         tmn lc als)::EC) 
+                         gl fs Mem0); 
+      try solve [clear CIH_bFdefInf CIH_bInsnInf; eauto].
+      inv HbFdefInf.
+      apply CIH_bFdefInf with (fid:=fid)(l':=l')(ps':=ps')(cs':=cs')(tmn':=tmn')
+        (fa:=fa)(la:=la)(va:=va)(lb:=lb)(gvs:=gvs)(lc1:=lc1)(fptr:=fptr)(fv:=fv)
+        (lp:=lp)(lc:=lc)(fptrs0:=fptrs) in H6; auto.
+
+  assert (forall state tr, 
+          bopInf state tr -> 
+          sop_diverges state tr) as bopInf__implies__sop_diverges.
+    cofix CIH_bopInf.
+    intros state tr0 HbopInf.
+    inversion HbopInf; subst.
+    Case "bopInf_insn".
+      apply bInsnInf__implies__sop_diverges in H; auto.
+    Case "bopInf_cons".
+      apply bInsn__implies__sop_plus in H.
+      inversion H; subst.
+      SCase "dsop_plus_cons".
+        apply CIH_bopInf in H0. clear CIH_bopInf.
+        apply sop_diverges_intro with (state2:=state2); auto.
+
+  intros fv rt lp S TD Ps ECs lc gl fs Mem0 tr fid fa lc1 l' ps' cs' tmn' la va 
+    lb gvs fptrs0 fptr Hin Hlookup HgetEntryBlock Hp2gvs Hinit HbFdefInf Hget.
+  inversion HbFdefInf; subst; eauto.
+Qed.
+
+Lemma bFdefInf__implies__sop_diverges : forall fv rt lp S TD Ps ECs lc gl fs Mem
+    tr fptrs,
+  bFdefInf fv rt lp S TD Ps ECs lc gl fs Mem tr ->
+  getOperandValue TD fv lc gl = Some fptrs -> 
+  exists fptr, exists fa, exists fid, exists la, exists va, exists lb, 
+  exists l', exists ps', exists cs', exists tmn', exists gvs, exists lc0, 
+  fptr @ fptrs /\
+  lookupFdefViaPtr Ps fs fptr = 
+    Some (fdef_intro (fheader_intro fa rt fid la va) lb) /\
+  getEntryBlock (fdef_intro (fheader_intro fa rt fid la va) lb) = 
+    Some (block_intro l' ps' cs' tmn') /\
+  params2GVs TD lp lc gl = Some gvs /\
+  initLocals TD la gvs = Some lc0 /\
+  sop_diverges 
+    (mkState S TD Ps ((mkEC (fdef_intro (fheader_intro fa rt fid la va) lb) 
+                        (block_intro l' ps' cs' tmn') cs' tmn' lc0
+                        nil)::ECs) gl fs Mem)
+    tr.
+Proof.
+  intros fv rt lp S TD Ps ECs lc gl fs Mem0 tr fptrs HdbFdefInf Hget.
+  inv HdbFdefInf; subst.
+  exists fptr. exists fa. exists fid. exists la. exists va. exists lb. exists l'.
+  exists ps'. exists cs'. exists tmn'. exists gvs. exists lc1.
+  rewrite Hget in H. inv H.
+  repeat (split; auto).
+    eapply bFdefInf_bopInf__implies__sop_diverges; eauto.
+Qed.
+
+Lemma bInsnInf__implies__sop_diverges : forall state tr, 
+  bInsnInf state tr -> sop_diverges state tr.
+Proof.
+  cofix CIH_bInsnInf.
+  intros state tr HbInsnInf.
+    
+  inversion HbInsnInf; subst.
+  rewrite <- nil_app_Trace__eq__Trace.
+  assert (HbFdefInf:=H).
+  inversion H; subst.
+  apply sop_diverges_intro with 
+    (state2:=mkState S TD Ps 
+                     ((mkEC (fdef_intro (fheader_intro fa rt fid la va) lb)
+                             (block_intro l' ps' cs' tmn') cs' tmn' lc1
+                             nil)::
+                      (mkEC F B ((insn_call rid noret0 ca ft fv lp)::cs) tmn
+                       lc als)::EC) 
+                       gl fs Mem0); 
+    try solve [clear CIH_bInsnInf; eauto].
+    eapply bFdefInf_bopInf__implies__sop_diverges with (l':=l')(ps':=ps')
+      (cs':=cs')(tmn':=tmn')(la:=la)(va:=va)(lb:=lb)(fa:=fa)(gvs:=gvs)(lc1:=lc1) 
+      in H6; eauto.
+Qed.
+
+Lemma bopInf__implies__sop_diverges : forall state tr, 
+  bopInf state tr -> sop_diverges state tr.
+Proof.
+  cofix CIH_bopInf.
+  intros state tr HdbopInf.
+  inversion HdbopInf; subst.
+  Case "bopInf_insn".
+    apply bInsnInf__implies__sop_diverges in H; auto.
+  Case "bopInf_cons".
+    apply bInsn__implies__sop_plus in H.
+    inversion H; subst.
+    SCase "sop_plus_cons".
+      apply CIH_bopInf in H0. clear CIH_bopInf.
+      apply sop_diverges_intro with (state2:=state2); auto.
+Qed.
+
+(** Then we prove that the whole program holds the same property. *)
+
+Lemma b_diverges__implies__s_diverges : forall sys main VarArgs tr, 
+  b_diverges sys main VarArgs tr ->
+  s_diverges sys main VarArgs tr.
+Proof.
+  intros sys main VarArgs tr Hdb_diverges.
+  inversion Hdb_diverges; subst.
+  apply s_diverges_intro with (IS:=IS)(tr:=tr); auto.
+  apply bopInf__implies__sop_diverges; auto.
+Qed.
+
+End OpsemConv.
+
 Module OpsemProps (GVsSig : GenericValuesSig).
 
 Module OS := Opsem GVsSig.
@@ -266,6 +779,567 @@ Proof.
   simpl in H. exists i0. eauto.
 Qed.  
 *)
+
+Lemma eqAL_callUpdateLocals : forall TD noret0 rid oResult lc1 lc2 gl lc1' 
+  lc2' ft,
+  eqAL _ lc1 lc1' ->
+  eqAL _ lc2 lc2' ->
+  match (callUpdateLocals TD ft noret0 rid oResult lc1 lc2 gl,
+         callUpdateLocals TD ft noret0 rid oResult lc1' lc2' gl) with
+  | (Some lc, Some lc') => eqAL _ lc lc'
+  | (None, None) => True
+  | _ => False
+  end.
+Proof.
+  intros TD noret0 rid oResult lc1 lc2 gl lc1' lc2' ft H1 H2.
+    unfold callUpdateLocals.
+    destruct noret0; auto.
+      destruct oResult; simpl; auto.
+        destruct v; simpl.
+          rewrite H2.
+          destruct (lookupAL _ lc2' i0); auto using eqAL_updateAddAL.
+
+          destruct (const2GV TD gl c); auto using eqAL_updateAddAL.
+      destruct oResult; simpl; auto.
+        destruct v; simpl.
+          rewrite H2.
+          destruct (lookupAL _ lc2' i0); auto.
+          destruct ft; auto.
+          destruct (GVsSig.lift_op1 (fit_gv TD ft) t ft); auto using eqAL_updateAddAL.
+
+          destruct (const2GV TD gl c); auto using eqAL_updateAddAL.
+          destruct ft; auto.
+          destruct (GVsSig.lift_op1 (fit_gv TD ft) g ft); auto using eqAL_updateAddAL.
+Qed.
+
+Lemma eqAL_getIncomingValuesForBlockFromPHINodes : forall TD ps B gl lc lc',
+  eqAL _ lc lc' ->
+  getIncomingValuesForBlockFromPHINodes TD ps B gl lc = 
+  getIncomingValuesForBlockFromPHINodes TD ps B gl lc'.
+Proof.
+  induction ps; intros; simpl; auto.
+    destruct a; auto.
+    destruct (getValueViaBlockFromValuels l0 B); auto.
+    destruct v; simpl; erewrite IHps; eauto.
+      rewrite H. auto.
+Qed.
+  
+Lemma eqAL_updateValuesForNewBlock : forall vs lc lc',
+  eqAL _ lc lc' ->
+  eqAL _ (updateValuesForNewBlock vs lc) (updateValuesForNewBlock vs lc').
+Proof.
+  induction vs; intros; simpl; auto.
+    destruct a; auto using eqAL_updateAddAL.
+Qed.
+
+Lemma eqAL_switchToNewBasicBlock : forall TD B1 B2 gl lc lc',
+  eqAL _ lc lc' ->
+  match (switchToNewBasicBlock TD B1 B2 gl lc,
+         switchToNewBasicBlock TD B1 B2 gl lc') with
+  | (Some lc1, Some lc1') => eqAL _ lc1 lc1'
+  | (None, None) => True
+  | _ => False
+  end.
+Proof.
+  intros.
+  unfold switchToNewBasicBlock.
+  erewrite eqAL_getIncomingValuesForBlockFromPHINodes; eauto.
+  destruct 
+    (getIncomingValuesForBlockFromPHINodes TD (getPHINodesFromBlock B1) B2 gl 
+    lc'); auto using eqAL_updateValuesForNewBlock.
+Qed.
+
+Lemma eqAL_params2GVs : forall lp TD lc gl lc',
+  eqAL _ lc lc' ->
+  params2GVs TD lp lc gl = params2GVs TD lp lc' gl.
+Proof.
+  induction lp; intros; simpl; auto.
+    destruct a. 
+    destruct v; simpl.
+      rewrite H. erewrite IHlp; eauto.
+      erewrite IHlp; eauto.
+Qed.
+
+Lemma eqAL_exCallUpdateLocals : forall TD noret0 rid oResult lc lc' ft,
+  eqAL _ lc lc' ->
+  match (exCallUpdateLocals TD ft noret0 rid oResult lc,
+         exCallUpdateLocals TD ft noret0 rid oResult lc') with
+  | (Some lc1, Some lc1') => eqAL _ lc1 lc1'
+  | (None, None) => True
+  | _ => False
+  end.
+Proof.
+  intros TD noret0 rid oResult lc lc' ft H1.
+    unfold exCallUpdateLocals.
+    destruct noret0; auto.
+    destruct oResult; auto.
+    destruct ft; auto.
+    destruct (fit_gv TD ft g); auto using eqAL_updateAddAL.
+Qed.
+
+Lemma updateValuesForNewBlock_uniq : forall l0 lc,
+  uniq lc ->
+  uniq (updateValuesForNewBlock l0 lc).
+Proof.
+  induction l0; intros lc Uniqc; simpl; auto.
+    destruct a; apply updateAddAL_uniq; auto.
+Qed.
+
+Lemma switchToNewBasicBlock_uniq : forall TD B1 B2 gl lc lc',
+  uniq lc ->
+  switchToNewBasicBlock TD B1 B2 gl lc = Some lc' ->
+  uniq lc'.
+Proof.
+  intros TD B1 B2 gl lc lc' Uniqc H.
+  unfold switchToNewBasicBlock in H.
+  destruct (getIncomingValuesForBlockFromPHINodes TD (getPHINodesFromBlock B1)
+    B2 gl lc); inversion H; subst.
+  apply updateValuesForNewBlock_uniq; auto.
+Qed.      
+
+Lemma initializeFrameValues_init : forall TD la l0 lc,
+  _initializeFrameValues TD la l0 nil = Some lc ->
+  uniq lc.
+Proof.
+  induction la; intros; simpl in *; auto.
+    inv H. auto.
+
+    destruct a as [[t ?] id0].
+    destruct l0.
+      remember (_initializeFrameValues TD la nil nil) as R.
+      destruct R; tinv H.
+      destruct (gundef TD t); inv H; eauto using updateAddAL_uniq.
+
+      remember (_initializeFrameValues TD la l0 nil) as R.
+      destruct R; tinv H.
+      destruct (GVsSig.lift_op1 (fit_gv TD t) g t); inv H; 
+        eauto using updateAddAL_uniq.
+Qed.
+
+Lemma initLocals_uniq : forall TD la ps lc,
+  initLocals TD la ps = Some lc -> uniq lc.
+Proof.
+  intros la ps.
+  unfold initLocals.
+  apply initializeFrameValues_init; auto.
+Qed.
+
+Lemma getIncomingValuesForBlockFromPHINodes_eq : 
+  forall ps TD l1 ps1 cs1 tmn1 ps2 cs2 tmn2,
+  getIncomingValuesForBlockFromPHINodes TD ps (block_intro l1 ps1 cs1 tmn1) =
+  getIncomingValuesForBlockFromPHINodes TD ps (block_intro l1 ps2 cs2 tmn2).
+Proof.
+  induction ps; intros; auto.
+    simpl.
+    erewrite IHps; eauto.
+Qed.
+
+Lemma switchToNewBasicBlock_eq : 
+  forall TD B l1 ps1 cs1 tmn1 ps2 cs2 tmn2 gl lc,
+  switchToNewBasicBlock TD B (block_intro l1 ps1 cs1 tmn1) gl lc =
+  switchToNewBasicBlock TD B (block_intro l1 ps2 cs2 tmn2) gl lc.
+Proof.
+  intros.
+  unfold switchToNewBasicBlock.
+  erewrite getIncomingValuesForBlockFromPHINodes_eq; eauto.
+Qed.
+
+Lemma bop_trans : forall state1 state2 state3 tr1 tr2,
+  bop state1 state2 tr1 ->
+  bop state2 state3 tr2 ->
+  bop state1 state3 (trace_app tr1 tr2).
+Proof.
+  intros state1 state2 state3 tr1 tr2 H.
+  generalize dependent state3.
+  generalize dependent tr2.
+  induction H; intros; auto.
+    rewrite <- trace_app_commute. eauto.
+Qed.
+
+Lemma bInsn__bop : forall state1 state2 tr,
+  bInsn state1 state2 tr ->
+  bop state1 state2 tr.
+Proof.
+  intros.
+  rewrite <- trace_app_nil__eq__trace.
+  eauto.
+Qed.
+
+Lemma bInsn__inv : forall S1 TD1 Ps1 F1 l1 ps1 cs1 tmn1 c cs tmn3 lc1 als1 
+    ECs1 gl1 fs1 Mem1 S2 TD2 Ps2 F2 l2 ps2 cs2 tmn2 tmn4 lc2 als2 ECs2 gl2 
+    fs2 Mem2 tr,
+  bInsn 
+    (mkState S1 TD1 Ps1 (mkEC F1 (block_intro l1 ps1 cs1 tmn1) (c::cs) tmn3 lc1 
+      als1::ECs1) gl1 fs1 Mem1) 
+    (mkState S2 TD2 Ps2 (mkEC F2 (block_intro l2 ps2 cs2 tmn2) cs tmn4 lc2
+      als2::ECs2) gl2 fs2 Mem2)
+    tr ->
+  S1 = S2 /\ TD1 = TD2 /\ Ps1 = Ps2 /\ F1 = F2 /\ l1 = l2 /\ ps1 = ps2 /\
+  cs1 = cs2 /\ tmn1 = tmn2 /\ tmn3 = tmn4 /\ gl1 = gl2 /\ fs1 = fs2.
+Proof.
+  intros.
+  inversion H; subst; repeat (split; auto).
+Qed.
+
+Lemma bInsn_Call__inv : forall S1 TD1 Ps1 F1 l1 ps1 cs1 tmn1 c cs tmn3 lc1 
+    als1 ECs1 gl1 fs1 Mem1 S2 TD2 Ps2 F2 l2 ps2 cs2 tmn2 tmn4 lc2 als2 ECs2
+     gl2 fs2 Mem2 tr,
+  bInsn 
+    (mkState S1 TD1 Ps1 (mkEC F1 (block_intro l1 ps1 cs1 tmn1) (c::cs) tmn3 lc1 
+      als1::ECs1) gl1 fs1 Mem1) 
+    (mkState S2 TD2 Ps2 (mkEC F2 (block_intro l2 ps2 cs2 tmn2) cs tmn4 lc2 
+      als2::ECs2) gl2 fs2 Mem2)
+    tr ->
+  Instruction.isCallInst c = true ->
+  S1 = S2 /\ TD1 = TD2 /\ Ps1 = Ps2 /\ F1 = F2 /\ l1 = l2 /\ ps1 = ps2 /\
+  cs1 = cs2 /\ tmn1 = tmn2 /\ tmn3 = tmn4 /\ gl1 = gl2  /\ fs1 = fs2 /\ 
+  als1 = als2.
+Proof.
+  intros.
+  inversion H; subst; try solve [inversion H0 | repeat (split; auto)].
+Qed.
+
+Lemma lookupFdefViaPtr_uniq : forall los nts Ps fs S fptr F,
+  uniqSystem S ->
+  moduleInSystem (module_intro los nts Ps) S ->
+  lookupFdefViaPtr Ps fs fptr = Some F ->
+  uniqFdef F.
+Proof.
+  intros.
+  apply lookupFdefViaPtr_inversion in H1.
+  destruct H1 as [fn [J1 J2]].
+  apply lookupFdefViaIDFromProducts_inv in J2; auto.
+  apply uniqSystem__uniqProducts in H0; auto.
+  eapply uniqProducts__uniqFdef; simpl; eauto.
+Qed.
+
+Lemma entryBlockInSystemBlockFdef'' : forall los nts Ps fs fv F S B,
+  moduleInSystem (module_intro los nts Ps) S ->
+  lookupFdefViaPtr Ps fs fv = Some F ->
+  getEntryBlock F = Some B ->
+  blockInSystemModuleFdef B S (module_intro los nts Ps) F.
+Proof.
+  intros.
+  apply lookupFdefViaPtr_inversion in H0.
+  destruct H0 as [fn [J1 J2]].
+  apply lookupFdefViaIDFromProducts_inv in J2.
+  apply entryBlockInFdef in H1.  
+  apply blockInSystemModuleFdef_intro; auto.
+Qed.
+
+(* preservation of uniqueness and inclusion *)
+
+Definition bInsn_preservation_prop state1 state2 tr
+  (db:bInsn state1 state2 tr) :=
+  forall S los nts Ps F l ps cs tmn lc als ECs gl fs Mem cs0,
+  state1 = (mkState S (los, nts) Ps ((mkEC F (block_intro l ps cs0 tmn) cs tmn 
+    lc als)::ECs) gl fs Mem) ->
+  uniqSystem S ->
+  blockInSystemModuleFdef (block_intro l ps cs0 tmn) S 
+    (module_intro los nts Ps) F ->
+  exists l', exists ps', exists cs', exists tmn', 
+  exists lc', exists als', exists Mem', exists cs0',
+  state2 = (mkState S (los, nts) Ps ((mkEC F (block_intro l' ps' cs0' tmn') cs' 
+    tmn' lc' als')::ECs) gl fs Mem') /\
+  blockInSystemModuleFdef (block_intro l' ps' cs0' tmn') S 
+    (module_intro los nts Ps) F.
+Definition bop_preservation_prop state1 state2 tr
+  (db:bop state1 state2 tr) :=
+  forall S los nts Ps F l ps cs tmn lc als ECs gl fs Mem l' ps' cs' tmn' lc'
+    als' gl' fs' Mem' cs0 cs0',
+  state1 = (mkState S (los, nts) Ps ((mkEC F (block_intro l ps cs0 tmn) cs tmn 
+    lc als)::ECs) gl fs Mem) ->
+  state2 = (mkState S (los, nts) Ps ((mkEC F (block_intro l' ps' cs0' tmn') cs' 
+    tmn' lc' als')::ECs) gl' fs' Mem') ->
+  uniqSystem S ->
+  blockInSystemModuleFdef (block_intro l ps cs0 tmn) S 
+    (module_intro los nts Ps) F ->
+  blockInSystemModuleFdef (block_intro l' ps' cs0' tmn') S 
+    (module_intro los nts Ps) F.
+Definition bFdef_preservation_prop fv rt lp S TD Ps ECs lc gl fs Mem lc' als' 
+  Mem' B' Rid oResult tr
+  (db:bFdef fv rt lp S TD Ps ECs lc gl fs Mem lc' als' Mem' B' Rid oResult tr) 
+  :=
+  forall los nts,
+  TD = (los, nts) ->
+  uniqSystem S ->
+  moduleInSystem (module_intro los nts Ps) S ->
+  exists fptrs, exists fptr, exists F, 
+    getOperandValue TD fv lc gl = Some fptrs /\
+    fptr @ fptrs /\ 
+    lookupFdefViaPtr Ps fs fptr = Some F /\
+    uniqFdef F /\
+    blockInSystemModuleFdef B' S (module_intro los nts Ps) F.
+
+Lemma b_preservation : 
+  (forall state1 state2 tr db, @bInsn_preservation_prop state1 state2 tr db) /\
+  (forall state1 state2 tr db, @bop_preservation_prop state1 state2 tr  db) /\
+  (forall fv rt lp S TD Ps lc gl fs Mem lc' als' Mem' B' Rid oResult tr ECs db, 
+    @bFdef_preservation_prop fv rt lp S TD Ps lc gl fs Mem lc' als' Mem' B' Rid 
+      oResult tr ECs db).
+Proof.
+(b_mutind_cases
+  apply b_mutind with
+    (P  := bInsn_preservation_prop)
+    (P0 := bop_preservation_prop)
+    (P1 := bFdef_preservation_prop) Case);
+  unfold bInsn_preservation_prop, 
+         bop_preservation_prop, 
+         bFdef_preservation_prop; intros; subst.
+Case "bBranch".
+  inversion H; subst. clear H.
+  exists l'. exists ps'. exists cs'. exists tmn'.
+  exists lc'. exists als0. exists Mem1.
+  exists cs'. split; auto.
+  apply andb_true_iff in H1.
+  destruct H1.
+  eapply andb_true_iff.
+  split; auto.
+    assert (uniqFdef F0) as UniqF0.
+      eapply uniqSystem__uniqFdef with (S:=S0); eauto.
+    symmetry in e0.
+    destruct (isGVZero (los, nts) c);
+      apply lookupBlockViaLabelFromFdef_inv in e0;
+      destruct e0; auto.
+
+Case "bBranch_uncond".
+  inversion H; subst. clear H.
+  exists l'. exists ps'. exists cs'. exists tmn'.
+  exists lc'. exists als0. exists Mem1.
+  exists cs'. split; auto.
+  apply andb_true_iff in H1.
+  destruct H1.
+  eapply andb_true_iff.
+  split; auto.
+    assert (uniqFdef F0) as UniqF0.
+      eapply uniqSystem__uniqFdef with (S:=S0); eauto.
+    symmetry in e.
+    apply lookupBlockViaLabelFromFdef_inv in e; auto.
+    destruct e; auto.
+
+Case "bBop".
+  inversion H; subst.
+  exists l0. exists ps. exists cs. exists tmn0.
+  exists (updateAddAL _ lc0 id0 gv3). exists als0. exists Mem1.
+  exists cs1. split; auto.
+
+Case "bFBop".
+  inversion H; subst.
+  exists l0. exists ps. exists cs. exists tmn0.
+  exists (updateAddAL _ lc0 id0 gv3). exists als0. exists Mem1.
+  exists cs1. split; auto.
+
+Case "bExtractValue".
+  inversion H; subst.
+  exists l0. exists ps. exists cs. exists tmn0.
+  exists (updateAddAL _ lc0 id0 gv'). exists als0. exists Mem1.
+  exists cs1. split; auto.
+
+Case "bInsertValue".
+  inversion H; subst.
+  exists l0. exists ps. exists cs. exists tmn0.
+  exists (updateAddAL _ lc0 id0 gv''). exists als0. exists Mem1.
+  exists cs1. split; auto.
+
+Case "bMalloc".
+  inversion H; subst.
+  exists l0. exists ps. exists cs. exists tmn0.
+  exists (updateAddAL _ lc0 id0 ($ blk2GV (los, nts) mb # typ_pointer t $)). 
+  exists als0. exists Mem'. exists cs1. split; auto.
+
+Case "bFree".
+  inversion H; subst. 
+  exists l0. exists ps. exists cs. exists tmn0.
+  exists lc0. exists als0. exists Mem'.
+  exists cs1. split; auto.
+
+Case "bAlloca".
+  inversion H; subst. 
+  exists l0. exists ps. exists cs. exists tmn0.
+  exists (updateAddAL _ lc0 id0 (($ blk2GV (los, nts) mb # typ_pointer t $))). 
+  exists (mb::als0). exists Mem'. exists cs1. split; auto.
+
+Case "bLoad".
+  inversion H; subst.
+  exists l0. exists ps. exists cs. exists tmn0.
+  exists (updateAddAL _ lc0 id0 ($ gv # t $)). exists als0. exists Mem1.
+  exists cs1. split; auto.
+
+Case "bStore".
+  inversion H; subst. 
+  exists l0. exists ps. exists cs. exists tmn0.
+  exists lc0. exists als0. exists Mem'.
+  exists cs1. split; auto.
+
+Case "bGEP".
+  inversion H; subst.
+  exists l0. exists ps. exists cs. exists tmn0.
+  exists (updateAddAL _ lc0 id0 mp'). exists als0. exists Mem1.
+  exists cs1. split; auto.
+
+Case "bTrunc".
+  inversion H; subst.
+  exists l0. exists ps. exists cs. exists tmn0.
+  exists (updateAddAL _ lc0 id0 gv2). exists als0. exists Mem1.
+  exists cs1. split; auto.
+
+Case "bExt".
+  inversion H; subst.
+  exists l0. exists ps. exists cs. exists tmn0.
+  exists (updateAddAL _ lc0 id0 gv2). exists als0. exists Mem1.
+  exists cs1. split; auto.
+
+Case "bCast".
+  inversion H; subst.
+  exists l0. exists ps. exists cs. exists tmn0.
+  exists (updateAddAL _ lc0 id0 gv2). exists als0. exists Mem1.
+  exists cs1. split; auto.
+
+Case "bIcmp".
+  inversion H; subst.
+  exists l0. exists ps. exists cs. exists tmn0.
+  exists (updateAddAL _ lc0 id0 gv3). exists als0. exists Mem1.
+  exists cs1. split; auto.
+
+Case "bFcmp".
+  inversion H; subst.
+  exists l0. exists ps. exists cs. exists tmn0.
+  exists (updateAddAL _ lc0 id0 gv3). exists als0. exists Mem1.
+  exists cs1. split; auto.
+
+Case "bSelect".
+  inversion H; subst.
+  exists l0. exists ps. exists cs. exists tmn0.
+  exists (if isGVZero (los, nts) c 
+          then updateAddAL _ lc0 id0 gv2 else updateAddAL _ lc0 id0 gv1). 
+  exists als0. exists Mem1. exists cs1. split; auto.
+
+Case "bCall".
+  inversion H0; subst. clear H0.
+  exists l0. exists ps. exists cs. exists tmn0.
+  exists lc''. exists als0. exists Mem''.
+  exists cs1. split; auto.
+ 
+Case "bExCall".
+  inversion H; subst.
+  exists l0. exists ps. exists cs. exists tmn0.
+  exists lc'. exists als0. exists Mem'.
+  exists cs1. split; auto.
+
+Case "bop_nil".
+  inversion H0; subst. auto.
+  
+Case "bop_cons".
+  apply H with (cs1:=cs)(lc0:=lc)(als0:=als)(ECs0:=ECs)(gl0:=gl)
+    (fs0:=fs)(Mem:=Mem0) in H4; auto.
+  clear H.
+  destruct H4 as [l1 [ps1 [cs1 [tmn1 [lc1 [als1 [Mem1 [cs1' [EQ H4]]]]]]]]]; 
+    subst.
+  eapply H0; eauto.
+
+Case "bFdef_func".
+  exists fptrs. exists fptr.
+  exists (fdef_intro (fheader_intro fa rt fid la va) lb).
+  split; auto.
+  split; auto.
+  split; auto.
+  split.
+    eapply lookupFdefViaPtr_uniq; eauto.
+    eapply H with (lc'0:=lc')(cs'0:=nil)(als'0:=als')(gl':=gl)(fs':=fs)
+      (Mem'0:=Mem'); 
+      eauto using entryBlockInSystemBlockFdef''.   
+
+Case "bFdef_proc".
+  exists fptrs. exists fptr.
+  exists (fdef_intro (fheader_intro fa rt fid la va) lb).
+  split; auto.
+  split; auto.
+  split; auto.
+  split.
+    eapply lookupFdefViaPtr_uniq; eauto.
+    eapply H; eauto using entryBlockInSystemBlockFdef''.
+Qed.
+
+Lemma _bInsn_preservation : forall state2 tr S los nts Ps F l ps cs tmn lc als 
+  ECs gl fs Mem cs0,
+  bInsn ((mkState S (los, nts) Ps ((mkEC F (block_intro l ps cs0 tmn) cs tmn lc 
+    als)::ECs) gl fs Mem)) state2 tr ->
+  uniqSystem S ->
+  blockInSystemModuleFdef (block_intro l ps cs0 tmn) S (module_intro los nts Ps) 
+    F ->
+  exists l', exists ps', exists cs', exists tmn', 
+  exists lc', exists als', exists Mem', exists cs0',
+  state2 = (mkState S (los, nts) Ps ((mkEC F (block_intro l' ps' cs0' tmn') cs' 
+    tmn' lc' als')::ECs) gl fs Mem') /\
+  blockInSystemModuleFdef (block_intro l' ps' cs0' tmn') S 
+    (module_intro los nts Ps) F.
+Proof.
+  intros.
+  destruct b_preservation as [J _].
+  unfold bInsn_preservation_prop in J.
+  eapply J; eauto.
+Qed.
+
+Lemma bInsn_preservation : forall tr S los nts Ps F l ps cs tmn lc als ECs gl 
+    fs Mem cs0 l' ps'  cs' tmn' lc' als' gl' fs' Mem' cs0',
+  bInsn 
+    ((mkState S (los, nts) Ps 
+      ((mkEC F (block_intro l ps cs0 tmn) cs tmn lc als)::ECs) gl fs Mem)) 
+    (mkState S (los, nts) Ps 
+      ((mkEC F (block_intro l' ps' cs0' tmn') cs' tmn' lc' als')::ECs) gl' fs' 
+        Mem')
+    tr ->
+  uniqSystem S ->
+  blockInSystemModuleFdef (block_intro l ps cs0 tmn) S (module_intro los nts Ps)
+    F ->
+  blockInSystemModuleFdef (block_intro l' ps' cs0' tmn') S 
+    (module_intro los nts Ps) F.
+Proof.
+  intros.
+  apply _bInsn_preservation in H; auto.
+  destruct H as [l1 [ps1 [cs1 [tmn1 [lc1 [als1 [Mem1 [cs2 [J1 J2]]]]]]]]].
+  inversion J1; subst. clear J1. auto.  
+Qed.
+
+Lemma bop_preservation : forall tr S los nts Ps F l ps cs tmn lc als ECs gl
+    fs Mem l' ps' cs' tmn' lc' als' gl' fs' Mem' cs0 cs0',
+  bop 
+    (mkState S (los, nts) Ps 
+      ((mkEC F (block_intro l ps cs0 tmn) cs tmn lc als)::ECs) gl fs Mem)
+    (mkState S (los, nts) Ps 
+      ((mkEC F (block_intro l' ps' cs0' tmn') cs' tmn' lc' als')::ECs) gl' fs' 
+        Mem')
+    tr ->
+  uniqSystem S ->
+  blockInSystemModuleFdef (block_intro l ps cs0 tmn) S (module_intro los nts Ps)
+    F ->
+  blockInSystemModuleFdef (block_intro l' ps' cs0' tmn') S 
+    (module_intro los nts Ps) F.
+Proof.
+  intros.
+  destruct b_preservation as [_ [J _]].
+  unfold bop_preservation_prop in J.
+  eapply J; eauto.
+Qed.
+
+Lemma bFdef_preservation : forall fv rt lp S los nts Ps ECs lc gl fs Mem lc' 
+    als' Mem' B' Rid oResult tr,
+  bFdef fv rt lp S (los, nts) Ps ECs lc gl fs Mem lc' als' Mem' B' Rid oResult tr
+    ->
+  uniqSystem S ->
+  moduleInSystem (module_intro los nts Ps) S ->
+  exists fptrs, exists fptr, exists F, 
+    getOperandValue (los, nts) fv lc gl = Some fptrs /\
+    fptr @ fptrs /\ 
+    lookupFdefViaPtr Ps fs fptr = Some F /\
+    uniqFdef F /\
+    blockInSystemModuleFdef B' S (module_intro los nts Ps) F.
+Proof.
+  intros.
+  destruct b_preservation as [_ [_ J]].
+  unfold bFdef_preservation_prop in J.
+  eapply J; eauto.
+Qed.
 
 End OpsemProps.
 
